lunarlander_sl/BigStepParallel.thy
@@ -46,7 +46,7 @@ inductive combine_blocks :: "cname set \<Rightarrow> trace \<Rightarrow> trace \
    compat_rdy rdy1 rdy2 \<Longrightarrow>
    hist = (\<lambda>\<tau>\<in>{0..t}. ParState (hist1 \<tau>) (hist2 \<tau>)) \<Longrightarrow>
    rdy = merge_rdy rdy1 rdy2 \<Longrightarrow>
-   combine_blocks comms (WaitBlock t hist1 rdy1 # blks1) (WaitBlock t hist2 rdy2 # blks2)
+   combine_blocks comms (WaitBlock (t::real) hist1 rdy1 # blks1) (WaitBlock t hist2 rdy2 # blks2)
                   (WaitBlock t hist rdy # blks)"
 | combine_blocks_wait2:
   "combine_blocks comms blks1 (WaitBlock (t2 - t1) (\<lambda>\<tau>\<in>{0..t2-t1}. hist2 (\<tau> + t1)) rdy2 # blks2) blks \<Longrightarrow>
